extra/State.v
@@ -1,0 +1,1047 @@
+(**
+
+This file contains a representation of finite maps
+that may be used for representing a store. It also
+provides lemmas and tactics for reasoning about
+operations on the store (read, write, union).
+
+Author: Arthur Charguéraud.
+License: CC-by 4.0.
+
+*)
+
+Set Implicit Arguments.
+From TLC Require Import LibCore.
+
+
+(** The type [memory V] is essentially a finite map from locations to values,
+    where [V] denotes the type of values.
+
+    Type type [memory V] is represented as a pair of a map of type [loc -> option V]
+    and a proof that the domain of the map is finite and does not bind the null
+    value. The finiteness of the domain is witnessed by a list of keys such that
+    the map binds any key not in that list to [None].
+
+*)
+
+
+(* ********************************************************************** *)
+(** * Locations *)
+
+(** Representation of locations using natural numbers. *)
+
+Definition loc : Type := nat.
+
+(** Definition of the null location as the address zero. *)
+
+Definition null : loc := 0%nat.
+
+
+(* ********************************************************************** *)
+(** * Unconstrained maps *)
+
+(* ---------------------------------------------------------------------- *)
+(* ** Representation *)
+
+(** Type of partial functions from [loc] to [V], without constraints on the
+    domain. *)
+
+Definition map (V:Type) : Type :=
+  loc -> option V.
+
+
+(* ---------------------------------------------------------------------- *)
+(* ** Operations *)
+
+(** Disjoint union of two partial functions *)
+
+Definition map_union (V:Type) (f1 f2:map V) : map V :=
+  fun (x:loc) => match f1 x with
+           | Some y => Some y
+           | None => f2 x
+           end.
+
+(** Removal from a partial functions *)
+
+Definition map_remove (V:Type) (f:map V) (k:loc) : map V :=
+  fun (x:loc) => If x = k then None else f x.
+
+(** Finite domain of a partial function, without the null location *)
+
+Definition map_finite (V:Type) (f:map V) : Prop :=
+  exists (L:list loc), forall (x:loc), f x <> None -> mem x L.
+
+(** Disjointness of domain of two partial functions *)
+
+Definition map_disjoint (V:Type) (f1 f2:map V) : Prop :=
+  forall (x:loc), f1 x = None \/ f2 x = None.
+
+(** Compatibility of two partial functions on the intersection
+    of their domains (only for Separation Logic with RO-permissions) *)
+
+Definition map_agree (V:Type) (f1 f2:map V) : Prop :=
+  forall x v1 v2,
+  f1 x = Some v1 ->
+  f2 x = Some v2 ->
+  v1 = v2.
+
+(** Domain of a map (as a predicate) *)
+
+Definition map_indom (V:Type) (f:map V) : (loc->Prop) :=
+  fun (x:loc) => f x <> None.
+
+
+(* ---------------------------------------------------------------------- *)
+(** Properties *)
+
+Section MapOps.
+Variables (V:Type).
+Implicit Types f : map V.
+
+(** Symmetry of disjointness *)
+
+Lemma map_disjoint_sym :
+  sym (@map_disjoint V).
+Proof using.
+  introv H. unfolds map_disjoint. intros z. specializes H z. intuition.
+Qed.
+
+(** Commutativity of disjoint union *)
+
+Lemma map_union_comm : forall f1 f2,
+  map_disjoint f1 f2 ->
+  map_union f1 f2 = map_union f2 f1.
+Proof using.
+  introv H. unfold map.
+  extens. intros x. unfolds map_disjoint, map_union.
+  specializes H x. cases (f1 x); cases (f2 x); auto. destruct H; false.
+Qed.
+
+(** Finiteness of union *)
+
+Lemma map_union_finite : forall f1 f2,
+  map_finite f1 ->
+  map_finite f2 ->
+  map_finite (map_union f1 f2).
+Proof using.
+  introv [L1 F1] [L2 F2]. exists (L1 ++ L2). intros x M.
+  specializes F1 x. specializes F2 x. unfold map_union in M.
+  apply mem_app. destruct~ (f1 x).
+Qed.
+
+(** Finiteness of removal *)
+
+Definition map_remove_finite : forall x f,
+  map_finite f ->
+  map_finite (map_remove f x).
+Proof using.
+  introv [L F]. exists L. intros x' M.
+  specializes F x'. unfold map_remove in M. case_if~.
+Qed.
+
+End MapOps.
+
+
+(* ********************************************************************** *)
+(** * Finite maps *)
+
+(* ---------------------------------------------------------------------- *)
+(** Definition of the type of valid maps *)
+
+Inductive memory (V:Type) : Type := make {
+  memory_data :> map V;
+  memory_finite : map_finite memory_data; }.
+
+Arguments make [V].
+
+
+(* ---------------------------------------------------------------------- *)
+(** Operations *)
+
+(** Empty memory *)
+
+Program Definition empty (V:Type) : memory V :=
+  make (fun l => None) _.
+Next Obligation. exists (@nil loc); auto_false. Qed.
+
+Arguments empty {V}.
+
+(** Singleton memory *)
+
+Program Definition single V (x:loc) (v:V) : memory V :=
+  make (fun x' => If x = x' then Some v else None) _.
+Next Obligation.
+  exists (x::nil). intros. case_if. subst~.
+Qed.
+
+(** Union of memories *)
+
+Program Definition union V (h1 h2:memory V) : memory V :=
+  make (map_union h1 h2) _.
+Next Obligation. destruct h1. destruct h2. apply~ map_union_finite. Qed.
+
+Notation "h1 \+ h2" := (union h1 h2)
+   (at level 51, right associativity) : memory_scope.
+
+Open Scope memory_scope.
+
+(** Update of a memory *)
+
+Definition update V (h:memory V) (x:loc) (v:V) : memory V :=
+  union (single x v) h.
+  (* Note: the union operation first reads in the first argument. *)
+
+(** Read in a memory *)
+
+Definition read (V:Type) {IB:Inhab V} (h:memory V) (x:loc) : V :=
+  match memory_data h x with
+  | Some y => y
+  | None => arbitrary
+  end.
+
+(** Removal from a memory *)
+
+Program Definition remove V (h:memory V) (x:loc) : memory V :=
+  make (map_remove h x) _.
+Next Obligation. destruct h. apply~ map_remove_finite. Qed.
+
+(** Domain of a memory (as a predicate) *)
+
+Definition indom (V: Type) (h:memory V) : (loc->Prop) :=
+  map_indom h.
+
+
+(* ---------------------------------------------------------------------- *)
+(** Properties *)
+
+(** Inhabited type [memory] *)
+
+Global Instance Inhab_memory V : Inhab (memory V).
+Proof using. intros. applys Inhab_of_val (@empty V). Qed.
+
+(** Compatible memories (only for Separation Logic with RO-permissions) *)
+
+Definition agree V (h1 h2:memory V) :=
+  map_agree h1 h2.
+
+(** Disjoint memories *)
+
+Definition disjoint V (h1 h2 : memory V) : Prop :=
+  map_disjoint h1 h2.
+
+(** Three disjoint memories (not needed for basic separation logic) *)
+
+Definition disjoint_3 V (h1 h2 h3 : memory V) :=
+     disjoint h1 h2
+  /\ disjoint h2 h3
+  /\ disjoint h1 h3.
+
+(** Notation for disjointness *)
+
+Module NotationForFmapDisjoint.
+
+Notation "\# h1 h2" := (disjoint h1 h2)
+  (at level 40, h1 at level 0, h2 at level 0, no associativity) : memory_scope.
+
+Notation "\# h1 h2 h3" := (disjoint_3 h1 h2 h3)
+  (at level 40, h1 at level 0, h2 at level 0, h3 at level 0, no associativity)
+  : memory_scope.
+
+End NotationForFmapDisjoint.
+
+Import NotationForFmapDisjoint.
+
+
+(* ********************************************************************** *)
+(* * Lemmas about Fmap *)
+
+Section FmapProp.
+Variables (V:Type).
+Implicit Types f g h : memory V.
+Implicit Types x : loc.
+Implicit Types v : V.
+
+(* ---------------------------------------------------------------------- *)
+(* ** Equality *)
+
+Lemma make_eq : forall (f1 f2:map V) F1 F2,
+  (forall x, f1 x = f2 x) ->
+  make f1 F1 = make f2 F2.
+Proof using.
+  introv H. asserts: (f1 = f2). { unfold map. extens~. }
+  subst. fequals. (* note: involves proof irrelevance *)
+Qed.
+
+Lemma eq_inv_memory_data_eq : forall h1 h2,
+  h1 = h2 ->
+  forall x, memory_data h1 x = memory_data h2 x.
+Proof using. intros. fequals. Qed.
+
+Lemma memory_extens : forall h1 h2,
+  (forall x, memory_data h1 x = memory_data h2 x) ->
+  h1 = h2.
+Proof using. intros [f1 F1] [f2 F2] M. simpls. applys~ make_eq. Qed.
+
+
+(* ---------------------------------------------------------------------- *)
+(* ** Disjointness *)
+
+Lemma disjoint_sym : forall h1 h2,
+  \# h1 h2 ->
+  \# h2 h1.
+Proof using. intros [f1 F1] [f2 F2]. apply map_disjoint_sym. Qed.
+
+Lemma disjoint_comm : forall h1 h2,
+  \# h1 h2 = \# h2 h1.
+Proof using. lets: disjoint_sym. extens*. Qed.
+
+Lemma disjoint_empty_l : forall h,
+  \# empty h.
+Proof using. intros [f F] x. simple~. Qed.
+
+Lemma disjoint_empty_r : forall h,
+  \# h empty.
+Proof using. intros [f F] x. simple~. Qed.
+
+Hint Resolve disjoint_sym disjoint_empty_l disjoint_empty_r.
+
+Lemma disjoint_union_eq_r : forall h1 h2 h3,
+  \# h1 (h2 \+ h3) =
+  (\# h1 h2 /\ \# h1 h3).
+Proof using.
+  intros [f1 F1] [f2 F2] [f3 F3].
+  unfolds disjoint, union. simpls.
+  unfolds map_disjoint, map_union. extens. iff M [M1 M2].
+  split; intros x; specializes M x;
+   destruct (f2 x); intuition; tryfalse.
+  intros x. specializes M1 x. specializes M2 x.
+   destruct (f2 x); intuition.
+Qed.
+
+Lemma disjoint_union_eq_l : forall h1 h2 h3,
+  \# (h2 \+ h3) h1 =
+  (\# h1 h2 /\ \# h1 h3).
+Proof using.
+  intros. rewrite disjoint_comm.
+  apply disjoint_union_eq_r.
+Qed.
+
+Lemma disjoint_single_single : forall x1 x2 v1 v2,
+  x1 <> x2 ->
+  \# (single x1 v1) (single x2 v2).
+Proof using.
+  introv N. intros x. simpls. do 2 case_if; auto.
+Qed.
+
+Lemma disjoint_single_single_same_inv : forall x v1 v2,
+  \# (single x v1) (single x v2) ->
+  False.
+Proof using.
+  introv D. specializes D x. simpls. case_if. destruct D; tryfalse.
+Qed.
+
+Lemma disjoint_3_unfold : forall h1 h2 h3,
+  \# h1 h2 h3 = (\# h1 h2 /\ \# h2 h3 /\ \# h1 h3).
+Proof using. auto. Qed.
+
+Lemma disjoint_single_set : forall h l v1 v2,
+  \# (single l v1) h ->
+  \# (single l v2) h.
+Proof using.
+  introv M. unfolds disjoint, single, map_disjoint; simpls.
+  intros l'. specializes M l'. case_if~. destruct M; auto_false.
+Qed.
+
+
+(* ---------------------------------------------------------------------- *)
+(* ** Union *)
+
+Lemma union_self : forall h,
+  h \+ h = h.
+Proof using.
+  intros [f F]. apply~ make_eq. simpl. intros x.
+  unfold map_union. cases~ (f x).
+Qed.
+
+Lemma union_empty_l : forall h,
+  empty \+ h = h.
+Proof using.
+  intros [f F]. unfold union, map_union, empty. simpl.
+  apply~ make_eq.
+Qed.
+
+Lemma union_empty_r : forall h,
+  h \+ empty = h.
+Proof using.
+  intros [f F]. unfold union, map_union, empty. simpl.
+  apply make_eq. intros x. destruct~ (f x).
+Qed.
+
+Lemma union_eq_empty_inv_l : forall h1 h2,
+  h1 \+ h2 = empty ->
+  h1 = empty.
+Proof using.
+  intros (f1&F1) (f2&F2) M. inverts M as M.
+  applys make_eq. intros l.
+  unfolds map_union.
+  lets: fun_eq_1 l M.
+  cases (f1 l); auto_false.
+Qed.
+
+Lemma union_eq_empty_inv_r : forall h1 h2,
+  h1 \+ h2 = empty ->
+  h2 = empty.
+Proof using.
+  intros (f1&F1) (f2&F2) M. inverts M as M.
+  applys make_eq. intros l.
+  unfolds map_union.
+  lets: fun_eq_1 l M.
+  cases (f1 l); auto_false.
+Qed.
+
+Lemma union_comm_of_disjoint : forall h1 h2,
+  \# h1 h2 ->
+  h1 \+ h2 = h2 \+ h1.
+Proof using.
+  intros [f1 F1] [f2 F2] H. simpls. apply make_eq. simpl.
+  intros. rewrite~ map_union_comm.
+Qed.
+
+Lemma union_comm_of_agree : forall h1 h2,
+  agree h1 h2 ->
+  h1 \+ h2 = h2 \+ h1.
+Proof using.
+  intros [f1 F1] [f2 F2] H. simpls. apply make_eq. simpl.
+  intros l. specializes H l. unfolds map_union. simpls.
+  cases (f1 l); cases (f2 l); auto. fequals. applys* H.
+Qed.
+
+Lemma union_assoc : forall h1 h2 h3,
+  (h1 \+ h2) \+ h3 = h1 \+ (h2 \+ h3).
+Proof using.
+  intros [f1 F1] [f2 F2] [f3 F3]. unfolds union. simpls.
+  apply make_eq. intros x. unfold map_union. destruct~ (f1 x).
+Qed.
+
+(*
+Lemma union_eq_inv_of_disjoint : forall h2 h1 h1' : memory,
+  \# h1 h2 ->
+  agree h1' h2 ->
+  h1 \+ h2 = h1' \+ h2 ->
+  h1 = h1'.
+Proof using.
+  intros [f2 F2] [f1 F1] [f1' F1'] D D' E.
+  applys make_eq. intros x. specializes D x. specializes D' x.
+  lets E': eq_inv_memory_data_eq (rm E) x. simpls.
+  unfolds map_union.
+  cases (f1 x); cases (f2 x); try solve [cases (f1' x); destruct D; congruence ].
+  destruct D; try false.
+  rewrite H in E'. inverts E'.
+  cases (f1' x); cases (f1 x);
+    destruct D; try congruence.
+  false.
+    destruct D'; try congruence.
+Qed.
+*)
+
+Lemma union_eq_inv_of_disjoint : forall h2 h1 h1',
+  \# h1 h2 ->
+  \# h1' h2 ->
+  h1 \+ h2 = h1' \+ h2 ->
+  h1 = h1'.
+Proof using.
+  intros [f2 F2] [f1' F1'] [f1 F1] D D' E.
+  applys make_eq. intros x. specializes D x. specializes D' x.
+  lets E': eq_inv_memory_data_eq (rm E) x. simpls.
+  unfolds map_union.
+  cases (f1' x); cases (f1 x);
+    destruct D; try congruence;
+    destruct D'; try congruence.
+Qed.
+
+
+(* ---------------------------------------------------------------------- *)
+(* ** Compatibility *)
+
+Lemma agree_refl : forall h,
+  agree h h.
+Proof using.
+  intros h. introv M1 M2. congruence.
+Qed.
+
+Lemma agree_sym : forall f1 f2,
+  agree f1 f2 ->
+  agree f2 f1.
+Proof using.
+  introv M. intros l v1 v2 E1 E2.
+  specializes M l E1.
+Qed.
+
+Lemma agree_of_disjoint : forall h1 h2,
+  disjoint h1 h2 ->
+  agree h1 h2.
+Proof using.
+  introv HD. intros l v1 v2 M1 M2. destruct (HD l); false.
+Qed.
+
+Lemma agree_empty_l : forall h,
+  agree empty h.
+Proof using. intros h l v1 v2 E1 E2. simpls. false. Qed.
+
+Lemma agree_empty_r : forall h,
+  agree h empty.
+Proof using.
+  hint agree_sym, agree_empty_l. eauto.
+Qed.
+
+Lemma agree_union_l : forall f1 f2 f3,
+  agree f1 f3 ->
+  agree f2 f3 ->
+  agree (f1 \+ f2) f3.
+Proof using.
+  introv M1 M2. intros l v1 v2 E1 E2.
+  specializes M1 l. specializes M2 l.
+  simpls. unfolds map_union. cases (memory_data f1 l).
+  { inverts E1. applys* M1. }
+  { applys* M2. }
+Qed.
+
+Lemma agree_union_r : forall f1 f2 f3,
+  agree f1 f2 ->
+  agree f1 f3 ->
+  agree f1 (f2 \+ f3).
+Proof using.
+  hint agree_sym, agree_union_l. eauto.
+Qed.
+
+Lemma agree_union_lr : forall f1 g1 f2 g2,
+  agree g1 g2 ->
+  \# f1 f2 (g1 \+ g2) ->
+  agree (f1 \+ g1) (f2 \+ g2).
+Proof using.
+  introv M1 (M2a&M2b&M2c).
+  rewrite disjoint_union_eq_r in *.
+  applys agree_union_l; applys agree_union_r;
+    try solve [ applys* agree_of_disjoint ].
+  auto.
+Qed.
+
+Lemma agree_union_ll_inv : forall f1 f2 f3,
+  agree (f1 \+ f2) f3 ->
+  agree f1 f3.
+Proof using.
+  introv M. intros l v1 v2 E1 E2.
+  specializes M l. simpls. unfolds map_union.
+  rewrite E1 in M. applys* M.
+Qed.
+
+Lemma agree_union_rl_inv : forall f1 f2 f3,
+  agree f1 (f2 \+ f3) ->
+  agree f1 f2.
+Proof using.
+  hint agree_union_ll_inv, agree_sym. eauto.
+Qed.
+
+Lemma agree_union_lr_inv_agree_agree : forall f1 f2 f3,
+  agree (f1 \+ f2) f3 ->
+  agree f1 f2 ->
+  agree f2 f3.
+Proof using.
+  introv M D. rewrite~ (@union_comm_of_agree f1 f2) in M.
+  applys* agree_union_ll_inv.
+Qed.
+
+Lemma agree_union_rr_inv_agree : forall f1 f2 f3,
+  agree f1 (f2 \+ f3) ->
+  agree f2 f3 ->
+  agree f1 f3.
+Proof using.
+  hint agree_union_lr_inv_agree_agree, agree_sym. eauto.
+Qed.
+
+Lemma agree_union_l_inv : forall f1 f2 f3,
+  agree (f1 \+ f2) f3 ->
+  agree f1 f2 ->
+     agree f1 f3
+  /\ agree f2 f3.
+Proof using.
+  introv M1 M2. split.
+  { applys* agree_union_ll_inv. }
+  { applys* agree_union_lr_inv_agree_agree. }
+Qed.
+
+Lemma agree_union_r_inv : forall f1 f2 f3,
+  agree f1 (f2 \+ f3) ->
+  agree f2 f3 ->
+     agree f1 f2
+  /\ agree f1 f3.
+Proof using.
+  hint agree_sym.
+  intros. forwards~ (M1&M2): agree_union_l_inv f2 f3 f1.
+Qed.
+
+
+(* ---------------------------------------------------------------------- *)
+(* ** Domain *)
+
+Lemma indom_single : forall x v,
+  indom (single x v) x.
+Proof using.
+  intros. hnf. simpl. case_if. auto_false.
+Qed.
+
+Lemma indom_union_l : forall h1 h2 x,
+  indom h1 x ->
+  indom (union h1 h2) x.
+Proof using.
+  intros. hnf. unfold union, map_union. simpl.
+  case_eq (memory_data h1 x); auto_false.
+Qed.
+
+Lemma indom_union_r : forall h1 h2 x,
+  indom h2 x ->
+  indom (union h1 h2) x.
+Proof using.
+  intros. hnf. unfold union, map_union. simpl.
+  case_eq (memory_data h1 x); auto_false.
+Qed.
+
+
+(* ---------------------------------------------------------------------- *)
+(* ** Disjoint and domain *)
+
+Lemma disjoint_eq_not_indom_both : forall h1 h2,
+  disjoint h1 h2 = (forall x, indom h1 x -> indom h2 x -> False).
+Proof using.
+  extens. iff D E.
+  { introv M1 M2. destruct (D x); false*. }
+  { intros x. specializes E x. unfolds indom, map_indom.
+    applys not_not_inv. intros N. rew_logic in N. false*. }
+Qed.
+
+Lemma disjoint_of_not_indom_both : forall h1 h2,
+  (forall x, indom h1 x -> indom h2 x -> False) ->
+  disjoint h1 h2.
+Proof using. introv M. rewrite~ disjoint_eq_not_indom_both. Qed.
+
+Lemma disjoint_inv_not_indom_both : forall h1 h2 x,
+  disjoint h1 h2 ->
+  indom h1 x ->
+  indom h2 x ->
+  False.
+Proof using. introv. rewrite* disjoint_eq_not_indom_both. Qed.
+
+Lemma disjoint_single_of_not_indom : forall h x v,
+  ~ indom h x ->
+  disjoint (single x v) h.
+Proof using.
+  introv N. unfolds disjoint, map_disjoint. unfolds single, indom, map_indom.
+  simpl. rew_logic in N. intros l'. case_if; subst; autos*.
+Qed.
+
+(* Remark: the reciprocal of the above lemma is a special instance of
+   [disjoint_inv_not_indom_both] *)
+
+
+(* ---------------------------------------------------------------------- *)
+(* ** Read *)
+
+Lemma read_single : forall {IB:Inhab V} x v,
+  read (single x v) x = v.
+Proof using.
+  intros. unfold read, single. simpl. case_if~.
+Qed.
+
+Lemma read_union_l : forall {IB:Inhab V} h1 h2 x,
+  indom h1 x ->
+  read (union h1 h2) x = read h1 x.
+Proof using.
+  intros. unfold read, union, map_union. simpl.
+  case_eq (memory_data h1 x); auto_false.
+Qed.
+
+Lemma read_union_r : forall {IB:Inhab V} h1 h2 x,
+  ~ indom h1 x ->
+  read (union h1 h2) x = read h2 x.
+Proof using.
+  intros. unfold read, union, map_union. simpl.
+  case_eq (memory_data h1 x).
+  { intros v Hv. false H. auto_false. }
+  { auto_false. }
+Qed.
+
+
+(* ---------------------------------------------------------------------- *)
+(* ** Update *)
+
+Lemma update_eq_union_single : forall h x v,
+  update h x v = union (single x v) h.
+Proof using. auto. Qed.
+
+Lemma update_single : forall h x v w,
+  update (single x v) x w = single x w.
+Proof using.
+  intros. rewrite update_eq_union_single.
+  applys make_eq. intros y.
+  unfold map_union, single. simpl. case_if~.
+Qed.
+
+Lemma update_union_l : forall h1 h2 x v,
+  indom h1 x ->
+  update (union h1 h2) x v = union (update h1 x v) h2.
+Proof using.
+  intros. do 2 rewrite update_eq_union_single.
+  applys make_eq. intros y.
+  unfold map_union, union, map_union. simpl. case_if~.
+Qed.
+
+Lemma update_union_r : forall h1 h2 x v,
+  ~ indom h1 x ->
+  update (union h1 h2) x v = union h1 (update h2 x v).
+Proof using.
+  introv M. asserts IB: (Inhab V). { applys Inhab_of_val v. }
+  do 2 rewrite update_eq_union_single.
+  applys make_eq. intros y.
+  unfold map_union, union, map_union. simpl. case_if~.
+  { subst. case_eq (memory_data h1 y); auto_false.
+    { intros w Hw. false M. auto_false. } }
+Qed.
+
+
+(* ---------------------------------------------------------------------- *)
+(* ** Removal *)
+
+Lemma remove_union_single_l : forall h x v,
+  ~ indom h x ->
+  remove (union (single x v) h) x = h.
+Proof using.
+  introv M. applys memory_extens. intros y.
+  unfold remove, map_remove, union, map_union, single. simpls. case_if.
+  { destruct h as [f F]. unfolds indom, map_indom. simpls. subst. rew_logic~ in M. }
+  { case_if~. }
+Qed.
+
+End FmapProp.
+
+
+(* ---------------------------------------------------------------------- *)
+(* ** Arguments *)
+
+Arguments union_assoc [V].
+Arguments union_comm_of_disjoint [V].
+Arguments union_comm_of_agree [V].
+
+
+(* ********************************************************************** *)
+(* * Tactics *)
+
+(* ---------------------------------------------------------------------- *)
+(* ** Tactic [disjoint] for proving disjointness results *)
+
+(** [disjoint] proves goals of the form [\# h1 h2] and
+    [\# h1 h2 h3] by expanding all hypotheses into binary forms
+    [\# h1 h2] and then exploiting symmetry and disjointness
+    with [empty]. *)
+
+Module Export DisjointHints.
+Hint Resolve disjoint_sym disjoint_empty_l disjoint_empty_r.
+End DisjointHints.
+
+Hint Rewrite
+  disjoint_union_eq_l
+  disjoint_union_eq_r
+  disjoint_3_unfold : rew_disjoint.
+
+Tactic Notation "rew_disjoint" :=
+  autorewrite with rew_disjoint in *.
+Tactic Notation "rew_disjoint" "*" :=
+  rew_disjoint; auto_star.
+
+Tactic Notation "memory_disjoint" :=
+  solve [ subst; rew_disjoint; jauto_set; auto ].
+
+Lemma disjoint_demo : forall V (h1 h2 h3 h4 h5:memory V),
+  h1 = h2 \+ h3 ->
+  \# h2 h3 ->
+  \# h1 h4 h5 ->
+  \# h3 h2 h5 /\ \# h4 h5.
+Proof using.
+  intros. dup 2.
+  { subst. rew_disjoint. jauto_set. auto. auto. auto. auto. }
+  { memory_disjoint. }
+Qed.
+
+
+(* ---------------------------------------------------------------------- *)
+(* ** Tactic [eq] for proving equality of memories,
+      and tactic [rew_memory] to normalize memory expressions. *)
+
+Section StateEq.
+Variables (V:Type).
+Implicit Types h : memory V.
+
+(** [eq] proves equalities between unions of memories, of the form
+    [h1 \+ h2 \+ h3 \+ h4 = h1' \+ h2' \+ h3' \+ h4']
+    It attempts to discharge the disjointness side-conditions.
+    Disclaimer: it cancels heaps at depth up to 4, but no more. *)
+
+Lemma union_eq_cancel_1 : forall h1 h2 h2',
+  h2 = h2' ->
+  h1 \+ h2 = h1 \+ h2'.
+Proof using. intros. subst. auto. Qed.
+
+Lemma union_eq_cancel_1' : forall h1,
+  h1 = h1.
+Proof using. intros. auto. Qed.
+
+Lemma union_eq_cancel_2 : forall h1 h1' h2 h2',
+  \# h1 h1' ->
+  h2 = h1' \+ h2' ->
+  h1 \+ h2 = h1' \+ h1 \+ h2'.
+Proof using.
+  intros. subst. rewrite <- union_assoc.
+  rewrite (union_comm_of_disjoint h1 h1').
+  rewrite~ union_assoc. auto.
+Qed.
+
+Lemma union_eq_cancel_2' : forall h1 h1' h2,
+  \# h1 h1' ->
+  h2 = h1' ->
+  h1 \+ h2 = h1' \+ h1.
+Proof using.
+  intros. subst. apply~ union_comm_of_disjoint.
+Qed.
+
+Lemma union_eq_cancel_3 : forall h1 h1' h2 h2' h3',
+  \# h1 (h1' \+ h2') ->
+  h2 = h1' \+ h2' \+ h3' ->
+  h1 \+ h2 = h1' \+ h2' \+ h1 \+ h3'.
+Proof using.
+  intros. subst.
+  rewrite <- (union_assoc h1' h2' h3').
+  rewrite <- (union_assoc h1' h2' (h1 \+ h3')).
+  apply~ union_eq_cancel_2.
+Qed.
+
+Lemma union_eq_cancel_3' : forall h1 h1' h2 h2',
+  \# h1 (h1' \+ h2') ->
+  h2 = h1' \+ h2' ->
+  h1 \+ h2 = h1' \+ h2' \+ h1.
+Proof using.
+  intros. subst.
+  rewrite <- (union_assoc h1' h2' h1).
+  apply~ union_eq_cancel_2'.
+Qed.
+
+Lemma union_eq_cancel_4 : forall h1 h1' h2 h2' h3' h4',
+  \# h1 ((h1' \+ h2') \+ h3') ->
+  h2 = h1' \+ h2' \+ h3' \+ h4' ->
+  h1 \+ h2 = h1' \+ h2' \+ h3' \+ h1 \+ h4'.
+Proof using.
+  intros. subst.
+  rewrite <- (union_assoc h1' h2' (h3' \+ h4')).
+  rewrite <- (union_assoc h1' h2' (h3' \+ h1 \+ h4')).
+  apply~ union_eq_cancel_3.
+Qed.
+
+Lemma union_eq_cancel_4' : forall h1 h1' h2 h2' h3',
+  \# h1 (h1' \+ h2' \+ h3') ->
+  h2 = h1' \+ h2' \+ h3' ->
+  h1 \+ h2 = h1' \+ h2' \+ h3' \+ h1.
+Proof using.
+  intros. subst.
+  rewrite <- (union_assoc h2' h3' h1).
+  apply~ union_eq_cancel_3'.
+Qed.
+
+End StateEq.
+
+Hint Rewrite
+  union_assoc
+  union_empty_l
+  union_empty_r : rew_memory.
+
+Tactic Notation "rew_memory" :=
+  autorewrite with rew_memory in *.
+
+Tactic Notation "rew_memory" "~" :=
+  rew_memory; auto_tilde.
+
+Tactic Notation "rew_memory" "*" :=
+  rew_memory; auto_star.
+
+Ltac memory_eq_step tt :=
+  match goal with | |- ?G => match G with
+  | ?h1 = ?h1 => apply union_eq_cancel_1'
+  | ?h1 \+ ?h2 = ?h1 \+ ?h2' => apply union_eq_cancel_1
+  | ?h1 \+ ?h2 = ?h1' \+ ?h1 => apply union_eq_cancel_2'
+  | ?h1 \+ ?h2 = ?h1' \+ ?h1 \+ ?h2' => apply union_eq_cancel_2
+  | ?h1 \+ ?h2 = ?h1' \+ ?h2' \+ ?h1 => apply union_eq_cancel_3'
+  | ?h1 \+ ?h2 = ?h1' \+ ?h2' \+ ?h1 \+ ?h3' => apply union_eq_cancel_3
+  | ?h1 \+ ?h2 = ?h1' \+ ?h2' \+ ?h3' \+ ?h1 => apply union_eq_cancel_4'
+  | ?h1 \+ ?h2 = ?h1' \+ ?h2' \+ ?h3' \+ ?h1 \+ ?h4' => apply union_eq_cancel_4
+  end end.
+
+Tactic Notation "memory_eq" :=
+  subst;
+  rew_memory;
+  repeat (memory_eq_step tt);
+  try match goal with
+  | |- \# _ _ => memory_disjoint
+  | |- \# _ _ _ => memory_disjoint
+  end.
+
+Tactic Notation "memory_eq" "~" :=
+  memory_eq; auto_tilde.
+
+Tactic Notation "memory_eq" "*" :=
+  memory_eq; auto_star.
+
+Lemma memory_eq_demo : forall V (h1 h2 h3 h4 h5:memory V),
+  \# h1 h2 h3 ->
+  \# (h1 \+ h2 \+ h3) h4 h5 ->
+  h1 = h2 \+ h3 ->
+  h4 \+ h1 \+ h5 = h2 \+ h5 \+ h4 \+ h3.
+Proof using.
+  intros. dup 2.
+  { subst. rew_memory.
+    memory_eq_step tt. memory_disjoint.
+    memory_eq_step tt.
+    memory_eq_step tt. memory_disjoint. auto. }
+  { memory_eq. }
+Qed.
+
+
+
+(* ********************************************************************** *)
+(** * Consecutive locations and fresh locations *)
+
+(* ---------------------------------------------------------------------- *)
+(** ** Consecutive locations *)
+
+Fixpoint conseq (V:Type) (l:nat) (vs:list V) : memory V :=
+  match vs with
+  | nil => empty
+  | v::vs' => (single l v) \+ (conseq (S l) vs')
+  end.
+
+Lemma conseq_nil : forall V (l:nat),
+  conseq l (@nil V) = empty.
+Proof using. auto. Qed.
+
+Lemma conseq_cons : forall V (l:nat) (v:V) (vs:list V),
+  conseq l (v::vs) = (single l v) \+ (conseq (S l) vs).
+Proof using. auto. Qed.
+
+Opaque conseq.
+
+
+(* ---------------------------------------------------------------------- *)
+(** ** Properties of fresh consecutive locations *)
+
+(** These lemmas are useful to prove:
+    [forall h v, exists l, disjoint (single l v) h]. *)
+
+Definition loc_fresh_gen (L : list nat) :=
+  (1 + fold_right plus O L)%nat.
+
+Lemma loc_fresh_ind : forall l L,
+  mem l L ->
+  (l < loc_fresh_gen L)%nat.
+Proof using.
+  intros l L. unfold loc_fresh_gen.
+  induction L; introv M; inverts M; rew_listx.
+  { math. }
+  { forwards~: IHL. math. }
+Qed.
+
+Lemma loc_fresh_nat_ge : forall (L:list nat),
+  exists (l:nat), forall (i:nat), ~ mem (l+i)%nat L.
+Proof using.
+  intros L. exists (loc_fresh_gen L). intros i M.
+  lets: loc_fresh_ind M. math.
+Qed.
+
+Lemma loc_fresh_nat : forall (L:list nat),
+  exists (l:nat), ~ mem l L.
+Proof using.
+  intros L. forwards (l&P): loc_fresh_nat_ge L.
+  exists l. intros M. applys (P 0%nat). applys_eq M 2. math.
+Qed.
+
+
+(* ---------------------------------------------------------------------- *)
+(** ** Extension of a number of consecutive fresh locations *)
+
+Section FmapFresh.
+Variables (V:Type).
+Implicit Types h : memory V.
+
+Lemma exists_not_indom : forall h,
+  exists l, ~ indom h l /\ l <> null.
+Proof using.
+  intros (m&(L&M)). unfold indom, map_indom. simpl.
+  lets (l&F): (loc_fresh_nat (null::L)).
+  exists l. split.
+  { simpl. intros l'. forwards~ E: M l. }
+  { intro_subst. applys~ F. }
+Qed.
+
+Lemma single_fresh : forall h v,
+  exists l, \# (single l v) h /\ l <> null.
+Proof using.
+  intros. forwards (l&F&N): exists_not_indom h.
+  exists l. split~. applys* disjoint_single_of_not_indom.
+Qed.
+
+Lemma conseq_fresh : forall null h k v,
+  exists l, \# (conseq l (LibList.make k v)) h /\ l <> null.
+Proof using.
+  intros null (m&(L&M)) k v.
+  unfold disjoint, map_disjoint. simpl.
+  lets (l&F): (loc_fresh_nat_ge (null::L)).
+  exists l. split.
+  { intros l'. gen l. induction k; intros.
+    { simple~. }
+    { rewrite make_succ. rewrite conseq_cons.
+      destruct (IHk (S l)%nat) as [E|?].
+      { intros i N. applys F (S i). applys_eq N 2. math. }
+      { simpl. unfold map_union. case_if~.
+        { subst. right. applys not_not_inv. intros H. applys F 0%nat.
+          constructor. math_rewrite (l'+0 = l')%nat. applys~ M. } }
+      { auto. } } }
+  { intro_subst. applys~ F 0%nat. rew_nat. auto. }
+Qed.
+
+Lemma disjoint_single_conseq : forall V l l' k (v:V),
+  (l < l')%nat \/ (l >= l'+k)%nat ->
+  \# (single l v) (conseq l' (LibList.make k v)).
+Proof using.
+  introv N. gen l'. induction k; intros.
+  { rewrite make_zero. rewrite~ conseq_nil. }
+  { rewrite make_succ. rewrite conseq_cons. rew_disjoint. split.
+    { applys disjoint_single_single. unfolds loc. destruct N; math. }
+    { applys IHk. destruct N. { left; math. } { right; math. } } }
+Qed.
+
+
+(* ---------------------------------------------------------------------- *)
+(* ** Existence of nonempty heaps *)
+
+(** This lemma is useful for constructing counterexamples. *)
+
+Lemma exists_not_empty : forall `{Inhab V},
+  exists (h:memory V), h <> empty.
+Proof using.
+  intros. sets l: 0%nat. sets h: (single l arbitrary).
+  exists h. intros N.
+  sets h': (empty:memory V).
+  asserts M1: (indom h l).
+  { applys indom_single. }
+  asserts M2: (~ indom h' l).
+  { unfolds @indom, map_indom, @empty. simpls. auto_false. }
+  rewrite N in M1. false*.
+Qed.
+
+End FmapFresh.
+
